Cslib/Logics/Propositional/Defs.lean
@@ -1,0 +1,46 @@
+/-
+Copyright (c) 2025 Thomas Waring. All rights reserved.
+Released under Apache 2.0 license as described in the file LICENSE.
+Authors: Thomas Waring
+-/
+import Mathlib.Order.Notation
+
+/-! # Propositions -/
+
+universe u
+
+variable {Atom : Type u} [DecidableEq Atom]
+
+namespace PL
+
+/-- Propositions. -/
+inductive Proposition (Atom : Type u) : Type u where
+  /-- Propositional atoms -/
+  | atom (x : Atom)
+  /-- Conjunction -/
+  | conj (a b : Proposition Atom)
+  /-- Disjunction -/
+  | disj (a b : Proposition Atom)
+  /-- Implication -/
+  | impl (a b : Proposition Atom)
+deriving DecidableEq, BEq
+
+instance instBotProposition [Bot Atom] : Bot (Proposition Atom) := ⟨.atom ⊥⟩
+instance instInhabitedOfBot [Bot Atom] : Inhabited Atom := ⟨⊥⟩
+
+/-- We view negation as a defined connective ~A := A → ⊥ -/
+abbrev Proposition.neg [Bot Atom] : Proposition Atom → Proposition Atom := (Proposition.impl · ⊥)
+
+/-- A fixed choice of a derivable proposition (of course any two are equivalent). -/
+def Proposition.top [Inhabited Atom] : Proposition Atom := impl (.atom default) (.atom default)
+
+instance instTopProposition [Inhabited Atom] : Top (Proposition Atom) := ⟨.top⟩
+
+example [Bot Atom] : (⊤ : Proposition Atom) = Proposition.impl ⊥ ⊥ := rfl
+
+@[inherit_doc] scoped infix:35 " ⋏ " => Proposition.conj
+@[inherit_doc] scoped infix:35 " ⋎ " => Proposition.disj
+@[inherit_doc] scoped infix:30 " ⟶ " => Proposition.impl
+@[inherit_doc] scoped prefix:40 " ~ " => Proposition.neg
+
+end PL
